\documentclass[10pt,a4paper]{letter}
\usepackage[latin1]{inputenc}
\usepackage{amsmath}
\usepackage{amsfonts}
\usepackage{amssymb}
\begin{document}
$$  \textit{P}_{E}(n,L) =\sum_{k=0}^{n-1}P(Last=k)\times(\textit{P}_{E}(k,k)\otimes\textit{P}_{E}(n-k-1,L-k-1))\\
$$

$$
Where:\textit{P}_{E}(A)\otimes\textit{P}_{E}(B) = \begin{cases}
\textit{P}_{E}(A)\times\textit{P}_{E}(B)+(1-\textit{P}_{E}(A))\times(1-\textit{P}_{E}(B)) 
& k:even\\
\textit{P}_{E}(A)\times(1-\textit{P}_{E}(B))+(1-\textit{P}_{E}(A))\times\textit{P}_{E}(B) 
& k:odd\\ 
\end{cases}
$$

\begin{align*}
& \text{and }P(Last=k)=\frac{L-k}{\sum_{k=0}^{N-1}(L-k)}\\
& \text{During the recursion we need only to compute 2N terms :}\\
& \textit{    - P}_{E}(k,k):k=0..N \text{ for the back race}\\
& \textit{    - P}_{E}(n,L-N+n):n=0..N \text{ for the front race}\\
& \text{Remark : In this explanation }L=1800/40	
\end{align*}

\end{document}