\documentclass[10pt,a4paper]{letter}
\usepackage[latin1]{inputenc}
\usepackage{amsmath}
\usepackage{amsfonts}
\usepackage{amssymb}
\begin{document}
$ - case\ A:\ \ \ L=\{2N-1,2N-1,2N\}$

$ (Py)\  (2N-1)^{2}=N^{2}+h^{2} $

$ \Rightarrow \exists\ m>n\ \  2N-1=m^{2}+n^{2}\ and\ N=m^{2}-n^{2}\ (1) $

$ other\ case\ N=2\times m \times n\ impossible\ due\ to\ \equiv 3 $

$ (1)\Rightarrow m^{2}=3\times n^{2}+1\Rightarrow \frac{n}{m} approximate \frac{1}{\sqrt{3}}	$

$With\ the\ continuous\ fraction\ for\ \frac{1}{\sqrt{3}}\ we\ found\ n,d\ \ d^{2}=n^{2}+1 $

$m=d\ ;N=m^{2}-n^{2}\ ;2N-1=m^{2}+n^{2}
\  ;h=2\times m\times n\ ;P=6N-2  $
$ - case\ B:\ \ \ L=\{2N+1,2N+1,2N\}$

$ (Py)\  (2N+1)^{2}=N^{2}+h^{2} $

$ \Rightarrow \exists\ m>n\ \  2N-1=m^{2}+n^{2}\ and\ N=2\times m \times n\ (2) $

$ other\ case\ N=m^{2}-n^{2}\ impossible\ due\ to\ \equiv 4 $

$ (2)\Rightarrow m^{2}+n^{2}-4m\times n=1 \Leftrightarrow (m-2n)^{2}=3\times n^{2} +1\Rightarrow \frac{n}{m-2n} approximate \frac{1}{\sqrt{3}}	$

$With\ the\ continuous\ fraction\ for\ \frac{1}{\sqrt{3}}\ we\ found\ n,d\ \ d^{2}=n^{2}+1 $

$m=d+2n\ ;N=2\times m\times n\ ;2N+1=m^{2}+n^{2}
\  ;h=m^{2}-n^{2}\ ;P=6N+2  $

$ P_{i}^{\alpha_{i}}\Rightarrow\frac{P_{i}^{\alpha_{i}}-1}{P_{i}-1} $

$\frac{k-1}{k+1}\times \binom{2k}{k} $

$ C(2n) = \sum_{k=2}^{k=n} \frac{k-1}{k+1}\times \binom{2k}{k} \times \binom{2n}{2k}$ 

$ P\rightarrow SumDiv[P]$
\end{document}
